HOTG/Cardinals/HOTG_Cardinals_Base.thy
@@ -4,10 +4,10 @@ section \<open>Cardinals\<close>
 theory HOTG_Cardinals_Base
   imports
     Transport.Binary_Relations_Least
+    HOTG_Ordinals_Equipollent
     HOTG_Equipollence
     HOTG_Ordinals_Base
     HOTG_Less_Than
-    HOTG_Choice
 begin
 
 unbundle no_HOL_groups_syntax
@@ -44,16 +44,15 @@ text\<open>The next lemma shows that @{term "|X|"} has the properties expected f
 lemma
   ordinal_cardinality: "ordinal |X|" and
   cardinality_equipollent_self [iff]: "|X| \<approx> X" and
-  cardinality_le_if_equipollent_ordinal: "\<forall>\<alpha> : ordinal. X \<approx> \<alpha> \<longrightarrow> |X| \<le> \<alpha>"
+  cardinality_le_if_equipollent_if_ordinal: "\<And>\<alpha>. ordinal \<alpha> \<Longrightarrow> X \<approx> \<alpha> \<Longrightarrow> |X| \<le> \<alpha>"
 proof -
   define P where "P \<equiv> ordinal \<sqinter> ((\<approx>) X)"
-  from equipollent_some_ordinal obtain \<alpha> where "ordinal \<alpha>" "X \<approx> \<alpha>" by blast
+  from bex_ordinal_equipollent obtain \<alpha> where "ordinal \<alpha>" "X \<approx> \<alpha>" by blast
   then have "P \<alpha>" "\<forall>\<beta> : P. ordinal \<beta>" using P_def by auto
-  then have least: "is_least_wrt_rel (\<le>) P |X|" 
-    using cardinality_def P_def least_ordinal_with_prop_welldefined_if_witness by auto
-  then show "ordinal |X|" "|X| \<approx> X" "\<forall>\<beta> : ordinal. X \<approx> \<beta> \<longrightarrow> |X| \<le> \<beta>" 
-    using P_def symmetric_equipollent 
-    by (auto elim!: is_least_wrt_relE is_minimal_wrt_relE dest: symmetricD)
+  then have least: "is_least_wrt_rel (\<le>) P |X|"
+    using cardinality_def P_def is_least_wrt_rel_least_wrt_rel_if_le_ordinal_if_pred by auto
+  then show "ordinal |X|" "|X| \<approx> X" "\<And>\<alpha>. ordinal \<alpha> \<Longrightarrow> X \<approx> \<alpha> \<Longrightarrow> |X| \<le> \<alpha>"
+    using P_def symmetric_equipollent by (blast dest: symmetricD)+
 qed
 
 lemma cardinality_cardinality_eq_cardinality [simp]: "||X|| = |X|"
@@ -69,7 +68,7 @@ proof -
   have "X \<approx> |X|" using cardinality_equipollent_self symmetric_equipollent by (blast dest: symmetricD)
   also have "... = |Y|" using assms by blast
   also have "... \<approx> Y" using cardinality_equipollent_self by blast
-  finally show ?thesis by blast
+  finally show ?thesis .
 qed
 
 corollary equipollent_iff_cardinality_eq: "X \<approx> Y \<longleftrightarrow> |X| = |Y|"
