HOTG/Ordinals/HOTG_Ordinals.thy
@@ -3,9 +3,10 @@
 theory HOTG_Ordinals
   imports
     HOTG_Ordinals_Base
+    HOTG_Ordinals_Equipollent
     HOTG_Ordinals_Max
+    HOTG_Ordinals_Omega
     HOTG_Ranks
-    HOTG_Natural_Numbers
 begin
 
 
